o Working on a "fresh" rule.

continuity/rules_fresh.v
@@ -31,6 +31,27 @@ Require Export subst_tacs_aeq.
 Require Export per_props_ffatom.
 
 
+Definition get_utokens_csub {o} (sub : @CSub o) :=
+  flat_map getc_utokens (crange sub).
+
+Lemma get_utokens_csub_as {o} :
+  forall (s : @CSub o),
+    get_utokens_csub s = get_utokens_sub (csub2sub s).
+Proof.
+  introv.
+  unfold get_utokens_csub, get_utokens_sub, crange, range, csub2sub.
+  rw map_map; unfold compose; simpl.
+  allrw flat_map_map; unfold compose; simpl; tcsp.
+Qed.
+
+Lemma cover_vars_uatom {o} :
+  forall (sub : @CSub o), cover_vars mk_uatom sub.
+Proof.
+  intro; rw @cover_vars_eq; rw subvars_eq; simpl; sp.
+Qed.
+Hint Resolve cover_vars_uatom : slow.
+
+
 (*
    H |- fresh(v.t) in T
 
@@ -48,11 +69,11 @@ Definition rule_fresh_member {o}
   mk_rule
     (mk_baresequent H (mk_conclax (mk_member (mk_fresh v t) T) ))
     [ mk_baresequent
-        (snoc (snoc H (mk_hyp a mk_uatom)) (mk_hyp z (mk_efree_from_atom mk_base (mk_fresh v t) (mk_var a))))
+        (snoc (snoc H (mk_hyp a mk_uatom)) (mk_hyp z (mk_free_from_atom mk_base (mk_fresh v t) (mk_var a))))
         (mk_conclax (mk_member (subst t v (mk_var a)) T)),
       mk_baresequent
-        (snoc (snoc H (mk_hyp a mk_uatom)) (mk_hyp z (mk_efree_from_atom mk_base (mk_fresh v t) (mk_var a))))
-        (mk_conclax (mk_efree_from_atom mk_base (subst t v (mk_var a)) (mk_var a))),
+        (snoc (snoc H (mk_hyp a mk_uatom)) (mk_hyp z (mk_free_from_atom mk_base (mk_fresh v t) (mk_var a))))
+        (mk_conclax (mk_free_from_atom mk_base (subst t v (mk_var a)) (mk_var a))),
       mk_baresequent H (mk_conclax (mk_member (mk_fresh v t) mk_base))
     ]
     [].
@@ -77,9 +98,12 @@ Proof.
   exists (@covered_axiom o (nh_vars_hyps H)).
 
   assert ((a <> v -> !LIn a (free_vars t))
+          # (z <> v -> !LIn z (free_vars t))
           # a <> z
           # !LIn a (vars_hyps H)
-          # !LIn z (vars_hyps H)) as vhyps.
+          # !LIn z (vars_hyps H)
+          # !LIn a (free_vars T)
+          # !LIn z (free_vars T)) as vhyps.
 
   {
     clear hyp1 hyp2 hyp3.
@@ -87,47 +111,234 @@ Proof.
     sp;
       try (complete (pose proof (ct2 a) as xx;
                      allrw in_remove_nvars; allsimpl;
+                     autodimp xx hyp; tcsp));
+      try (complete (pose proof (ct2 z) as xx;
+                     allrw in_remove_nvars; allsimpl;
                      autodimp xx hyp; tcsp)).
   }
 
   destruct vhyps as [ nat vhyps ].
+  destruct vhyps as [ nzt vhyps ].
   destruct vhyps as [ daz vhyps ].
-  destruct vhyps as [ naH nzH ].
+  destruct vhyps as [ naH vhyps ].
+  destruct vhyps as [ nzH vhyps ].
+  destruct vhyps as [ naT nzT ].
 
   vr_seq_true.
-  vr_seq_true in hyp3.
-
-  pose proof (hyp3 s1 s2 eqh sim) as hb; exrepnd.
   lsubst_tac.
   allrw <- @member_member_iff.
-  apply tequality_mkc_member_base in hb0; spcast.
-
-  pose proof (get_fresh_atom_prop t) as fa.
-  remember (get_fresh_atom t) as ua; clear Hequa.
 
   pose proof (teq_and_member_if_member
-                lib T (mk_fresh v t) s1 s2 H wT wt ct1 ct2 cT cT0)
+                lib T (mk_fresh v t) s1 s2 H wT wt ct2 ct3 cT cT0)
     as teq.
   repeat (autodimp teq hyp); auto;[| |lsubst_tac; auto].
 
-  - vr_seq_true in hyp1.
+  - destruct (fresh_atom o (get_utokens t ++ get_utokens_csub s1)) as [ua fa].
+    rw in_app_iff in fa; rw not_over_or in fa; repnd.
+
+    vr_seq_true in hyp1.
     pose proof (hyp1
                   (snoc (snoc s1 (a,mkc_utoken ua)) (z,mkc_axiom))
-                  (snoc (snoc s1 (a,mkc_utoken ua)) (z,mkc_axiom)))
+                  (snoc (snoc s2 (a,mkc_utoken ua)) (z,mkc_axiom)))
       as hyp; clear hyp1.
     repeat (autodimp hyp hh).
 
     + apply hyps_functionality_snoc2; simpl; auto.
 
       * introv equ' sim'.
+        apply similarity_snoc in sim'; exrepnd; cpx; ginv.
+        allsimpl.
         lsubst_tac.
-        apply tequality_efree_from_atom; dands; eauto 3 with slow.
+        apply tequality_free_from_atom; dands; eauto 3 with slow.
 
-        { pose proof (lsubstc_vars_csub_filter_snoc_ex t w1 s1 a (mkc_utoken ua) [v] c4) as equ.
-          rw in_single_iff in equ.
-          autodimp equ hyp; exrepnd.
-          rw equ0; clear equ0.
-        }
+        pose proof (lsubstc_vars_csub_filter_snoc_ex t w1 s1a a (mkc_utoken ua) [v] c4) as equ.
+        rw in_single_iff in equ.
+        autodimp equ hyp; exrepnd.
+        rw equ0; clear equ0.
+
+        pose proof (lsubstc_vars_csub_filter_snoc_ex t w1 s2a a t2 [v] c7) as equ.
+        rw in_single_iff in equ.
+        autodimp equ hyp; exrepnd.
+        rw equ0; clear equ0.
+
+        vr_seq_true in hyp3.
+        pose proof (hyp3 s1a s2a eqh sim'3) as hyp; clear hyp3; exrepnd.
+        lsubst_tac.
+        apply tequality_mkc_member_base in hyp0; spcast.
+        apply equality_in_base_iff; spcast; auto.
+
+      * apply hyps_functionality_snoc2; simpl; auto.
+        introv equ' sim'.
+        lsubst_tac.
+        apply tequality_uatom.
+
+    + sim_snoc2.
+
+      { apply wf_free_from_atom; eauto 2 with slow. }
+
+      { apply cover_vars_free_from_atom; dands; eauto 3 with slow;
+        try (complete (apply cover_vars_snoc_weak; auto)).
+        apply cover_vars_var_iff; rw @dom_csub_snoc; simpl; rw in_snoc; tcsp. }
+
+      dands; auto.
+
+      * sim_snoc2.
+        dands; auto.
+
+        lsubst_tac.
+        apply equality_in_uatom_iff.
+        exists ua; dands; spcast; apply computes_to_valc_refl; eauto 3 with slow.
+
+      * lsubst_tac.
+        apply equality_in_free_from_atom.
+
+        pose proof (lsubstc_vars_csub_filter_snoc_ex t w1 s1 a (mkc_utoken ua) [v] c4) as equ.
+        rw in_single_iff in equ.
+        autodimp equ hyp; exrepnd.
+        rw equ0; clear equ0.
+
+        exists (mkc_fresh v (lsubstc_vars t w1 (csub_filter s1 [v]) [v] cv')) ua.
+        dands; spcast; try (complete (apply computes_to_valc_refl; eauto 3 with slow));
+        try (apply tequality_base).
+
+        { apply equality_in_base_iff; spcast; eauto 3 with slow. }
+
+        unfold getc_utokens; simpl; autorewrite with slow.
+        intro i.
+        apply atoms2.get_utokens_lsubst_subset in i.
+        rw in_app_iff in i; repndors; tcsp;[].
+        rw @get_utokens_csub_as in fa.
+        rw <- @sub_filter_csub2sub in i.
+        allrw @in_get_utokens_sub.
+        exrepnd.
+        apply in_sub_filter in i0; repnd.
+        destruct fa.
+        exists v0 t0; dands; auto.
+
+    + exrepnd.
+      lsubst_tac.
+      apply tequality_mkc_member_sp in hyp0; repnd; auto.
+
+  - clear dependent s1.
+    clear dependent s2.
+
+    introv hf sim.
+    lsubst_tac.
+
+    assert (!LIn a (dom_csub s1)) as nias1.
+    { allapply @similarity_dom; repnd; allrw; auto. }
+
+    assert (!LIn z (dom_csub s1)) as nizs1.
+    { allapply @similarity_dom; repnd; allrw; auto. }
+
+    destruct (fresh_atom o (get_utokens t ++ get_utokens_csub s1 ++ get_utokens_csub s2)) as [ua fa].
+    repeat (rw in_app_iff in fa); repeat (rw not_over_or in fa); repnd.
+
+    vr_seq_true in hyp1.
+    pose proof (hyp1
+                  (snoc (snoc s1 (a,mkc_utoken ua)) (z,mkc_axiom))
+                  (snoc (snoc s2 (a,mkc_utoken ua)) (z,mkc_axiom)))
+      as hyp; clear hyp1.
+    repeat (autodimp hyp hh).
+
+    + apply hyps_functionality_snoc2; simpl; auto.
+
+      * introv equ' sim'.
+        apply similarity_snoc in sim'; exrepnd; cpx; ginv.
+        allsimpl.
+        lsubst_tac.
+        apply tequality_free_from_atom; dands; eauto 3 with slow.
+
+        pose proof (lsubstc_vars_csub_filter_snoc_ex t w1 s1a a (mkc_utoken ua) [v] c4) as equ.
+        rw in_single_iff in equ.
+        autodimp equ hyp; exrepnd.
+        rw equ0; clear equ0.
+
+        pose proof (lsubstc_vars_csub_filter_snoc_ex t w1 s2a a t2 [v] c7) as equ.
+        rw in_single_iff in equ.
+        autodimp equ hyp; exrepnd.
+        rw equ0; clear equ0.
+
+        vr_seq_true in hyp3.
+        pose proof (hyp3 s1a s2a hf sim'3) as hyp; clear hyp3; exrepnd.
+        lsubst_tac.
+        apply tequality_mkc_member_base in hyp0; spcast.
+        apply equality_in_base_iff; spcast; auto.
+
+      * apply hyps_functionality_snoc2; simpl; auto.
+        introv equ' sim'.
+        lsubst_tac.
+        apply tequality_uatom.
+
+    + sim_snoc2.
+
+      { apply wf_free_from_atom; eauto 2 with slow. }
+
+      { apply cover_vars_free_from_atom; dands; eauto 3 with slow;
+        try (complete (apply cover_vars_snoc_weak; auto)).
+        apply cover_vars_var_iff; rw @dom_csub_snoc; simpl; rw in_snoc; tcsp. }
+
+      dands; auto.
+
+      * sim_snoc2; eauto 3 with slow.
+        dands; auto.
+
+        lsubst_tac.
+        apply equality_in_uatom_iff.
+        exists ua; dands; spcast; apply computes_to_valc_refl; eauto 3 with slow.
+
+      * lsubst_tac.
+        apply equality_in_free_from_atom.
+
+        pose proof (lsubstc_vars_csub_filter_snoc_ex t w1 s1 a (mkc_utoken ua) [v] c4) as equ.
+        rw in_single_iff in equ.
+        autodimp equ hyp; exrepnd.
+        rw equ0; clear equ0.
+
+        exists (mkc_fresh v (lsubstc_vars t w1 (csub_filter s1 [v]) [v] cv')) ua.
+        dands; spcast; try (complete (apply computes_to_valc_refl; eauto 3 with slow));
+        try (apply tequality_base).
+
+        { apply equality_in_base_iff; spcast; eauto 3 with slow. }
+
+        unfold getc_utokens; simpl; autorewrite with slow.
+        intro i.
+        apply atoms2.get_utokens_lsubst_subset in i.
+        rw in_app_iff in i; repndors; tcsp;[].
+        rw @get_utokens_csub_as in fa1.
+        rw <- @sub_filter_csub2sub in i.
+        allrw @in_get_utokens_sub.
+        exrepnd.
+        apply in_sub_filter in i0; repnd.
+        destruct fa1.
+        exists v0 t0; dands; auto.
+
+    + exrepnd.
+      lsubst_tac.
+      allrw <- @member_member_iff.
+
+      vr_seq_true in hyp3.
+      pose proof (hyp3 s1 s2 hf sim) as hyp; clear hyp3; exrepnd.
+      clear hyp4.
+      lsubst_tac.
+      apply tequality_mkc_member_base in hyp3; spcast.
+      eapply equality_respects_cequivc_right;[eauto|].
+      rw @member_eq.
+      clear dependent s2.
+
+      assert (cover_vars (mk_var a) (snoc (snoc s1 (a, mkc_utoken ua)) (z, mkc_axiom))) as cova.
+      { apply cover_vars_var; allrw @dom_csub_snoc; simpl.
+        allrw in_snoc; tcsp. }
+
+      repeat (lsubstc_subst_aeq2;[]).
+      repeat (substc_lsubstc_vars3;[]).
+      lsubst_tac.
+
+      repeat (lsubstc_snoc2;[]).
+      GC; proof_irr; auto.
+
+
+Check cequivc_fresh_subst1.
 
 Qed.
 
